Fist theorem proven

doc/formalization/Catala.Translation.fst
@@ -5,6 +5,9 @@ module D = Catala.DefaultCalculus
 
 (*** Translation definitions *)
 
+
+(**** Helpers *)
+
 let rec translate_ty (ty: D.ty) : Tot L.ty = match ty with
   | D.TBool -> L.TBool
   | D.TUnit -> L.TUnit
@@ -18,19 +21,19 @@ let translate_lit (l: D.lit) : Tot L.lit = match l with
   | D.LConflictError -> L.LError L.ConflictError
 
 let process_exceptions_f (tau: L.ty) : Tot L.exp =
-  let a = -1 in
-  let e = -2 in
-  let e' = -3 in
-  let a' = -4 in
-  let e'' = -5 in
-  L.EAbs a (L.TOption tau) (L.EAbs e (L.TArrow L.TUnit tau) (
-    L.EApp (L.EAbs e' (L.TOption tau) (
+  let a = 0 in
+  let e = 1 in
+  let e' = 2 in
+  let a' = 3 in
+  let e'' = 4 in
+  L.EAbs (L.Named a) (L.TOption tau) (L.EAbs (L.Named e) (L.TArrow L.TUnit tau) (
+    L.EApp (L.EAbs (L.Named e') (L.TOption tau) (
       L.EMatchOption (L.EVar a) tau
         (L.EVar e')
-        (L.EAbs a' tau (
+        (L.EAbs (L.Named a') tau (
           L.EMatchOption (L.EVar e') tau
             (L.EVar a)
-            (L.EAbs e'' tau (L.ELit (L.LError L.ConflictError)))
+            (L.EAbs (L.Named e'') tau (L.ELit (L.LError L.ConflictError)))
         ))
     ))
     (L.ECatchEmptyError (L.ESome (L.EApp (L.EVar e) (L.ELit L.LUnit) L.TUnit)) L.ENone)
@@ -44,12 +47,29 @@ let typ_process_exceptions_f (tau: L.ty)
   assert_norm(L.typing L.empty (process_exceptions_f tau)
       (L.TArrow (L.TOption tau) (L.TArrow (L.TArrow L.TUnit tau) (L.TOption tau))))
 
+noeq type env' = {
+  tys: D.env;
+  max_free: nat
+}
+let env = g:env'{forall (i:nat{i > g.max_free}). g.tys i = None}
+
+let extend (g: env) (x: D.var) (ty: D.ty) : env =
+  let new_tys = D.extend g.tys x ty in
+  let new_max_free = if x > g.max_free then x else g.max_free in
+  { tys = new_tys; max_free = new_max_free }
+
+(**** Main translation *)
+
 let rec translate_exp (e: D.exp) : Tot L.exp = match e with
   | D.EVar x -> L.EVar x
-  | D.EApp e1 e2 tau_arg -> L.EApp (translate_exp e1) (translate_exp e2) (translate_ty tau_arg)
-  | D.EAbs x ty body -> L.EAbs x (translate_ty ty) (translate_exp body)
+  | D.EApp e1 e2 tau_arg ->
+    L.EApp (translate_exp e1) (translate_exp e2) (translate_ty tau_arg)
+  | D.EAbs x ty body -> L.EAbs (L.Named x) (translate_ty ty) (translate_exp body)
   | D.ELit l -> L.ELit (translate_lit l)
-  | D.EIf e1 e2 e3 -> L.EIf (translate_exp e1) (translate_exp e2) (translate_exp e3)
+  | D.EIf e1 e2 e3 -> L.EIf
+    (translate_exp e1)
+    (translate_exp e2)
+    (translate_exp e3)
   | D.EDefault exceptions just cons tau ->
     let tau' = translate_ty tau in
     L.EMatchOption
@@ -58,16 +78,20 @@ let rec translate_exp (e: D.exp) : Tot L.exp = match e with
         L.ENone (L.TOption tau')
         (L.EList (translate_exp_list exceptions)) (L.TArrow L.TUnit tau'))
       tau'
-      (L.EIf (translate_exp just) (translate_exp cons) (L.ELit (L.LError L.EmptyError)))
-      (L.EAbs (-1) tau' (L.EVar (-1)))
+      (L.EIf
+        (translate_exp just)
+        (translate_exp cons)
+        (L.ELit (L.LError L.EmptyError)))
+      (L.EAbs (L.Named 0) tau' (L.EVar 0))
 
-and translate_exp_list (l: list D.exp) : Tot (list L.exp) = match l with
+and translate_exp_list (l: list D.exp) : Tot (list L.exp) =
+  match l with
   | [] -> []
-  | hd::tl -> (L.EAbs (-1) L.TUnit (translate_exp hd))::(translate_exp_list tl)
+  | hd::tl -> (L.EAbs L.Silent L.TUnit (translate_exp hd))::(translate_exp_list tl)
 
 let translate_env (g: D.env) : Tot L.env =
- FunctionalExtensionality.on_dom L.var
-   (fun v -> if v < 0 then None else match g v with None -> None | Some t -> Some (translate_ty t))
+ FunctionalExtensionality.on_dom L.var_name
+   (fun v -> match g v with None -> None | Some t -> Some (translate_ty t))
 
 (*** Typing preservation *)
 
@@ -76,30 +100,9 @@ let translate_env (g: D.env) : Tot L.env =
 let extend_translate_commute (g: D.env) (x: D.var) (tau: D.ty)
     : Lemma (L.extend (translate_env g) x (translate_ty tau) == translate_env (D.extend g x tau))
   =
-  FunctionalExtensionality.extensionality L.var (fun _ -> option L.ty)
+  FunctionalExtensionality.extensionality L.var_name (fun _ -> option L.ty)
     (L.extend (translate_env g) x (translate_ty tau))
     (translate_env (D.extend g x tau))
-
-let rec typing_preserved_by_additional_lambda_variable
-  (g: D.env) (e: L.exp) (tau: L.ty) (v: L.var{v < 0}) (tv: L.ty)
-    : Lemma
-      (requires (L.typing (translate_env g) e tau))
-      (ensures (L.typing (L.extend (translate_env g) v tv) e tau))
-  =
-  let aux = typing_preserved_by_additional_lambda_variable in
-  match e with
-  | L.EVar v' -> ()
-  | L.EApp e1 e2 tau_arg ->
-    aux g e1 (L.TArrow tau_arg tau) v tv;
-    aux g e2 tau_arg v tv
-  | L.EAbs v' tau_arg body -> begin
-    match tau with
-    | L.TArrow tau_in tau_out ->
-      if tau_in <> tau_arg then () else
-      admit()
-    | _ -> ()
-  end
-  | _ -> admit()
 
 (**** Typing preservation theorem *)
 
@@ -107,7 +110,7 @@ let rec typing_preserved_by_additional_lambda_variable
 let rec translation_preserves_typ (g: D.env) (e: D.exp) (tau: D.ty) : Lemma
     (requires (D.typing g e tau))
     (ensures (L.typing (translate_env g) (translate_exp e) (translate_ty tau)))
-    (decreases %[e; 0])
+    (decreases %[e; 1])
   =
   match e with
   | D.EVar _ -> ()
@@ -128,10 +131,31 @@ let rec translation_preserves_typ (g: D.env) (e: D.exp) (tau: D.ty) : Lemma
     translation_preserves_typ g e1 D.TBool;
     translation_preserves_typ g e2 tau;
     translation_preserves_typ g e3 tau
-  | D.EDefault exceptions just cons tau' ->
-    if tau = tau' then
-      admit()
-    else ()
+  | D.EDefault exceptions just cons tau_out ->
+    if tau = tau_out then begin
+      let tau' = translate_ty tau in
+      translation_preserves_typ_exceptions g e exceptions tau;
+      typ_process_exceptions_f tau';
+      translation_preserves_typ g just D.TBool;
+      translation_preserves_typ g cons tau;
+      let result_exp = L.EMatchOption
+        (L.EFoldLeft
+          (process_exceptions_f tau')
+          L.ENone (L.TOption tau')
+          (L.EList (translate_exp_list exceptions)) (L.TArrow L.TUnit tau'))
+        tau'
+        (L.EIf
+          (translate_exp just)
+          (translate_exp cons)
+          (L.ELit (L.LError L.EmptyError)))
+        (L.EAbs (L.Named 0) tau' (L.EVar 0))
+      in
+      let open FStar.Tactics in
+      assert(L.typing (translate_env g) result_exp tau') by begin
+        compute ();
+        smt ()
+      end
+    end else ()
 and translation_preserves_typ_exceptions
   (g: D.env)
   (e: D.exp)
@@ -157,6 +181,5 @@ and translation_preserves_typ_exceptions
     let thunked_tau' = L.TArrow L.TUnit tau' in
     assert(L.typing_list g' tl' thunked_tau');
     assert(L.typing g' hd' tau');
-    typing_preserved_by_additional_lambda_variable g hd' tau' (-1) L.TUnit;
-    assert(L.typing g' (L.EAbs (-1) L.TUnit hd') thunked_tau')
+    assert(L.typing g' (L.EAbs L.Silent L.TUnit hd') thunked_tau')
 #pop-options
